Trying to switch the representation of labels from Type to Fin. The length of the change blew up in my hands, all of ktree has to be duplicated and adapted. Unfinished at the moment

tutorial/Asm.v
@@ -1,5 +1,3 @@
-(** * The Asm language  *)
-
 (** We now consider as a target a simple control-flow-graph language,
     so-called _Asm_.
     Computations are represented as a collection of basic blocks
@@ -13,11 +11,14 @@ From Coq Require Import
      ZArith.ZArith.
 
 From ITree Require Import
-     ITree.
+     Basics.Function
+     ITree
+     OpenSum
+     KTree.
 
 From ExtLib Require Structures.Monad.
 
-Require Import Imp.
+Require Import Imp Label.
 
 Typeclasses eauto := 5.
 
@@ -49,7 +50,7 @@ Variant instr : Set :=
 
 (** We consider both direct and conditional jumps *)
 Variant branch {label : Type} : Type :=
-| Bjmp (_ : label)                (* jump to label *)
+| Bjmp (_ : label) (* jump to label *)
 | Bbrz (_ : var) (yes no : label) (* conditional jump *)
 | Bhalt
 .
@@ -63,11 +64,12 @@ Inductive block {label : Type} : Type :=
 | bbb (_ : branch label).
 Global Arguments block _ : clear implicits.
 
-(** A piece of code should expose the set of labels allowing to enter
-    into it, as well as the set of outer labels it might jump to.
+(** A piece of code should expose the set of labels allowing
+    to enter into it, as well as the set of outer labels it might
+    jump to.
     To this end, [bks] represents a collection of blocks labeled
     by [A], with branches in [B]. *)
-Definition bks (A B: Type) := A -> block B.
+Definition bks A B := Fin.t A -> block (Fin.t B).
 
 (** An [asm] program represents the control flow of the computation.
     It is a collection of labelled [blocks] such that its labels are
@@ -79,10 +81,10 @@ Definition bks (A B: Type) := A -> block B.
     the latter corresponding to an [asm] program with a unique entry
     point and always halting, i.e. a [asm unit void].
  *)
-Record asm (A B: Type) : Type :=
+Record asm A B : Type :=
   {
-    internal : Type;
-    code : bks (internal + A) (internal + B)
+    internal : nat;
+    code     : bks (internal + A) (internal + B)
   }.
 
 Arguments internal {A B}.
@@ -91,10 +93,10 @@ Arguments code {A B}.
 (* ================================================================= *)
 (** ** Semantics *)
 
-(** _Asm_ produces two kind of events: through manipulation of the store
+(** _Asm_ produces two kind of effects: through manipulation of the store
     and of the heap.
     We therefore reuse _Imp_'s [Locals], and define an additional pair of
-    events [Memory] to model interactions with the heap.
+    effects [Memory].
 *)
 Import Imp.
 
@@ -104,7 +106,7 @@ Inductive Memory : Type -> Type :=
 
 Section Denote.
 
-  (** Once again, [asm] programs shall be denoted as [itree]s. *)
+  (** Once again, [asm] programs shall be deonted as [itree]s. *)
 
   (* begin hide *)
   Import ExtLib.Structures.Monad.
@@ -112,10 +114,10 @@ Section Denote.
   Local Open Scope monad_scope.
   (* end hide *)
 
-  (** We introduce a special event to model termination of the computation.
+  (** We introduce a special effect to model termination of the computation.
       Note that it expects _actively_ no answer from the environment: 
       [Done] is of type [Exit void].
-      We can therefore use it to "close" an [itree E A] no matter what the expected
+      We can therefore use it to close a [itree E A] no matter what the expected
       return type [A] is, as witnessed by the [done] computation.
    *)
   Inductive Exit : Type -> Type :=
@@ -124,9 +126,9 @@ Section Denote.
   Definition done {E A} `{Exit -< E} : itree E A :=
     vis Done (fun v => match v : void with end).
 
-  Section with_event.
+  Section with_effect.
 
-    (** As with _Imp_, we parameterize our semantics by a universe of events
+    (** As with _Imp_, we parameterize our semantics by a universe of effects
         that shall encompass all the required ones.
      *)
     Context {E : Type -> Type}.
@@ -138,7 +140,7 @@ Section Denote.
     Definition denote_operand (o : operand) : itree E value :=
       match o with
       | Oimm v => Ret v
-      | Ovar v => trigger (GetVar v)
+      | Ovar v => lift (GetVar v)
       end.
 
     (** Instructions offer no suprises either. *)
@@ -146,42 +148,42 @@ Section Denote.
       match i with
       | Imov d s =>
         v <- denote_operand s ;;
-        trigger (SetVar d v)
+        lift (SetVar d v)
       | Iadd d l r =>
-        lv <- trigger (GetVar l) ;;
+        lv <- lift (GetVar l) ;;
         rv <- denote_operand r ;;
-        trigger (SetVar d (lv + rv))
+        lift (SetVar d (lv + rv))
       | Isub d l r =>
-        lv <- trigger (GetVar l) ;;
+        lv <- lift (GetVar l) ;;
         rv <- denote_operand r ;;
-        trigger (SetVar d (lv - rv))
+        lift (SetVar d (lv - rv))
       | Imul d l r =>
-        lv <- trigger (GetVar l) ;;
+        lv <- lift (GetVar l) ;;
         rv <- denote_operand r ;;
-        trigger (SetVar d (lv * rv))
+        lift (SetVar d (lv * rv))
       | Iload d a =>
         addr <- denote_operand a ;;
-        val <- trigger (Load addr) ;;
-        trigger (SetVar d val)
+        val <- lift (Load addr) ;;
+        lift (SetVar d val)
       | Istore a v =>
-        addr <- trigger (GetVar a) ;;
+        addr <- lift (GetVar a) ;;
         val <- denote_operand v ;;
-        trigger (Store addr val)
+        lift (Store addr val)
       end.
 
     Section with_labels.
-      Context {A B : Type}.
+      Context {A B : nat}.
 
       (** A [branch] returns the computed label whose set of possible
           values [B] is carried by the type of the branch.
           If the computation halts instead of branching,
           we return the [done] tree.
        *)
-      Definition denote_branch (b : branch B) : itree E B :=
+      Definition denote_branch (b : branch (Fin.t B)) : itree E (Fin.t B) :=
         match b with
         | Bjmp l => ret l
         | Bbrz v y n =>
-          val <- trigger (GetVar v) ;;
+          val <- lift (GetVar v) ;;
           if val:nat then ret y else ret n
         | Bhalt => done
         end.
@@ -190,7 +192,7 @@ Section Denote.
           returning the [label] of the next [block] it shall jump to.
           It recursively denote its instruction before that.
        *)
-      Fixpoint denote_block (b : block B) : itree E B :=
+      Fixpoint denote_block (b : block (Fin.t B)) : itree E (Fin.t B) :=
         match b with
         | bbi i b =>
           denote_instr i ;; denote_block b
@@ -201,79 +203,83 @@ Section Denote.
       (** A labelled collection of blocks, [bks], is simply the pointwise
           application of [denote_block].
           However, its denotation is therefore crucially a [ktree],
-          whose structure will be useful in the proof of the compiler.
+          whose structure will be heavily taken profit of in the proof
+          of the compiler.
        *)
-      Definition denote_b (bs: bks A B): ktree E A B :=
+      Definition denote_b (bs: bks A B): ktree E (Fin.t A) (Fin.t B) :=
         fun a => denote_block (bs a).
 
     End with_labels.
 
-  (** One can think of an [asm] program as a circuit/diagram where wires
+  (** One can think of an asm program as a circuit/diagram where wires
       correspond to jumps/program links.
       [denote_b] computes the meaning of each basic block as an [itree] that
       returns the label of the next block to jump to, laying down all our
       elementary wires. 
       In order to denote an [asm A B] program as a [ktree E A B], it therefore
       remains to wire all those denoted blocks together while hiding the
-      internal labels.
-      Luckily, that is exactly what traced monoidal category are good for.
-      We therefore accomplish this with the same [loop] combinator we used to
-      denote _Imp_'s [while] loop.
+      internal lables.
+      We accomplish this with the same [loop] combinator we used to denote
+      _Imp_'s [while] loop.
       It directly takes our [denote_b (code s): ktree E (I + A) (I + B)] and
       hides [I] as desired.
    *)
 
     (* Denotation of [asm] *)
-    Definition denote_asm {A B} : asm A B -> ktree E A B :=
-      fun s => loop (denote_b (code s)).
 
-  End with_event.
+    Definition denote_asm {A B} : asm A B -> ktree E (Fin.t A) (Fin.t B) :=
+      fun s => loop_Label (denote_b (code s)).
+
+  End with_effect.
 End Denote.
 
 (* ================================================================= *)
 (** ** Interpretation *)
 
-(* begin hide *)
 From ITree Require Import
-     Basics.Category
-     Events.Map.
+     Effects.Env.
 
 From ExtLib Require Import
      Core.RelDec
      Structures.Maps
      Data.Map.FMapAList.
-(* end hide *)
 
-(** Both environments and memory events can be interpreted as "map" events,
+(** Both environments and memory effects can be interpreted as "map" effects,
     exactly as we did for _Imp_. *)
 
-Definition evalMemory {E : Type -> Type} `{mapE value value -< E} :
+Definition interpret_Locals {E : Type -> Type} `{envE var value -< E} :
+  Locals ~> itree E :=
+  fun _ e =>
+    match e with
+    | GetVar x => env_lookupDefault x 0
+    | SetVar x v => env_add x v
+    end.
+
+Definition interpret_Memory {E : Type -> Type} `{envE value value -< E} :
   Memory ~> itree E :=
   fun _ e =>
     match e with
-    | Load x => lookup_def x 0
-    | Store x v => insert x v
+    | Load x => env_lookupDefault x 0
+    | Store x v => env_add x v
     end.
 
 (** Once again, we implement our Maps with a simple association list *)
+Definition env := alist var value.
 Definition memory := alist value value.
 
-(** We can then define an evaluator for closed assembly programs by
-    interpreting both store and heap events into two instances of [mapE],
-    and running them both.
- *)
-Definition AsmEval (p: asm unit void) :=
-  let h := bimap evalLocals (bimap evalMemory (id_ _)) in
-  let p' := interp h (denote_asm p tt) in
-  run_map (run_map p' empty) empty.
+(* Enable typeclass instances for Maps keyed by strings and values *)
+Instance RelDec_string : RelDec (@eq string) :=
+  { rel_dec := fun s1 s2 => if String.string_dec s1 s2 then true else false}.
 
-(** Now that we have both our language, we could jump directly into implementing
-    our compiler.
-    However, if we look slightly ahead of us, we can observe that:
-    - compiling expressions and basic statements will be mostly straightforward;
-    - but linking the resulting elementary (open) [asm] programs together is not
-    as trivial. In particular, reasoning inductively on this linking is more
-    challenging.
-    We therefore take a detour: we first reason in isolation about linking, and
-    to this end we jump to [AsmCombinators.v].
- *)
+Instance RelDec_value : RelDec (@eq value) := { rel_dec := Nat.eqb }.
+
+(* TODO: redefine the interpreter *)
+(* Definition AsmEval (p: asm unit void): itree void1 (env * unit) := *)
+(*   let p := interp evalLocals _ (denoteStmt s) in *)
+(*   run_env _ p empty. *)
+(* Definition run (p: asm unit done) : itree emptyE (env * (memory * unit)) := *)
+(*   let eval := Sum1.elim interpret_Locals interpret_Memory in *)
+(*   run_env _ (run_env _ (interp eval _ (denote_asm p tt)) empty) empty. *)
+
+
+(**  *)
