tutorial/AsmCombinators.v
@@ -2,47 +2,38 @@
 
 (** We develop in this file a theory of linking for [asm] programs.
     To this end, we will equip them with four main combinators:
+    - [par_asm], linking them vertically
+    - [loop_asm], hiding internal links
+    - [relable_asm], allowing to rename labels
     - [pure_asm], casting pure functions into [asm]. 
-    - [app_asm], linking them vertically
-    - [link_asm], hiding internal links
-    - [relabel_asm], allowing to rename labels
-    Viewing [asm] units as diagrams, whose entry wires are the exposed labels of
-    its blocks, and exit wires the external labels to which it may jump, this
-    theory can be seen in particular as showing that they enjoy a structure of
-    _traced monoidal category_.
-    We do so by thinking of [ktree]s as a theory of linking at the denotational
-    level. Each linking combinator is therefore proved correct by showing that
-    the denotation of the resulting [asm], a [ktree],  can be swapped with the
-    corresponding [ktree] combinator.
-    It is interesting to notice that while the [ktree] theory, provided by the
-    library, required heavy use of coinduction, it provides sufficient reasoning
-    principles so that we do not need to write any cofix here.
+    Viewing [asm] units as diagrams, this theory can be seen in particular
+    as showing that they enjoy a structure of _traced monoidal category_ by
+    interpreting [ktree]s as a theory of linking at the denotational level.
+    Each linking combinator is therefore proved correct by showing that its
+    denotation can be swapped with the corresponding [ktree] combinator.
  *)
 
 (* begin hide *)
-Require Import Imp Asm Utils_tutorial.
+Require Import Asm Utils_tutorial Label LabelFacts.
 
 From Coq Require Import
      List
      Strings.String
      Program.Basics
+     Vectors.Fin
      ZArith.
 Import ListNotations.
 
 From ITree Require Import
-     ITree
-     ITreeFacts.
-
-From ExtLib Require Import
-     Structures.Monad.
+     Basics.Basics
+     Basics.Function
+     Basics.Category.
 
 Typeclasses eauto := 5.
 (* end hide *)
 
-(* ================================================================= *)
 (** ** Internal structures *)
 
-(** A utility function to apply a renaming function [f] to the exit label of a [branch]. *)
 Definition fmap_branch {A B : Type} (f: A -> B): branch A -> branch B :=
   fun b =>
     match b with
@@ -51,361 +42,356 @@ Definition fmap_branch {A B : Type} (f: A -> B): branch A -> branch B :=
     | Bhalt => Bhalt
     end.
 
-(** A utility function to apply a renaming function [f] to the exit label of a [block]. *)
 Definition fmap_block {A B: Type} (f: A -> B): block A -> block B :=
   fix fmap b :=
     match b with
     | bbb a => bbb (fmap_branch f a)
     | bbi i b => bbi i (fmap b)
     end.
-
-(** A utility function to apply renaming functions [f] and [g] respectively to
-    the entry and exit labels of a [bks]. *)
-Definition relabel_bks {A B C D : Type} (f : A -> B) (g : C -> D)
-           (b : bks B C) : bks A D :=
+         
+Definition relabel_bks {A B X D : nat} (f : FinC A B) (g : FinC X D)
+           (b : bks B X) : bks A D :=
   fun a => fmap_block g (b (f a)).
 
-(** Simple combinator to build a [block] from its instructions and branch operation. *)
 Fixpoint after {A: Type} (is : list instr) (bch : branch A) : block A :=
   match is with
   | nil => bbb bch
   | i :: is => bbi i (after is bch)
   end.
 
-(* ================================================================= *)
 (** ** Low-level interface with [asm] *)
 
 (** Any collection of blocks forms an [asm] program with no hidden blocks. *)
 Definition raw_asm {A B} (b : bks A B) : asm A B :=
-  {| internal := void;
-     code := fun a' =>
-               match a' with
-               | inl v => match v : void with end
-               | inr a => fmap_block inr (b a)
-               end;
+  {| internal := 0;
+     code := fun l => b l
   |}.
 
-(** And so does a single [block] in particular. *)
-Definition raw_asm_block {A} (b : block A) : asm unit A :=
+(** Wrap a single block as [asm]. *)
+Definition raw_asm_block {A: nat} (b : block (Fin.t A)) : asm 1 A :=
   raw_asm (fun _ => b).
 
 (** ** [asm] combinators *)
 
-(** We now turn to the proper [asm] combinators. *)
-
-(** An [asm] program made only of external jumps.
-    This is useful to connect programs with [app_asm]. *)
-Definition pure_asm {A B} (f : A -> B) : asm A B :=
+(** An [asm] program made only of external jumps. This is
+      useful to connect programs with [app_asm]. *)
+Definition pure_asm {A B: nat} (f : Fin.t A -> Fin.t B) : asm A B :=
   raw_asm (fun a => bbb (Bjmp (f a))).
 
 Definition id_asm {A} : asm A A := pure_asm id.
 
-(** The [app_asm] combinator joins two [asm] programs, 
-    preserving their internal links.
-    Since the three ambient domains of labels are extended,
-    the only tricky part is to rename all labels appropriately.
-    The two following functions take care of this internal
-    relabelling.
- *)
-Definition _app_B {I J B D} :
-  block (I + B) -> block ((I + J) + (B + D)) :=
+(* Internal relabeling functions for [app_asm] *)
+Definition _app_B {I J B D: nat} :
+  block (Fin.t (I + B)) -> block (Fin.t ((I + J) + (B + D))) :=
   fmap_block (fun l =>
-                match l with
-                | inl i => inl (inl i)
-                | inr b => inr (inl b)
+                match split_fin_sum l with
+                | inl i => L _ (L _ i)
+                | inr b => R _ (L _ b)
                 end).
 
 Definition _app_D {I J B D} :
-  block (J + D) -> block ((I + J) + (B + D)) :=
+  block (Fin.t (J + D)) -> block (Fin.t ((I + J) + (B + D))) :=
   fmap_block (fun l =>
-                match l with
-                | inl j => inl (inr j)
-                | inr d => inr (inr d)
+                match split_fin_sum l with
+                | inl j => L _ (R _ j)
+                | inr d => R _ (R _ d)
                 end).
 
-(** Combinator to append two asm programs, preserving their internal links.
-    Can be thought of as a "vertical composition", or a tensor product. 
- *)
+(** Append two asm programs, preserving their internal links. *)
 Definition app_asm {A B C D} (ab : asm A B) (cd : asm C D) :
   asm (A + C) (B + D) :=
   {| internal := ab.(internal) + cd.(internal);
      code := fun l =>
-               match l with
-               | inl (inl ia) => _app_B (ab.(code) (inl ia))
-               | inl (inr ic) => _app_D (cd.(code) (inl ic))
-               | inr (inl  a) => _app_B (ab.(code) (inr  a))
-               | inr (inr  c) => _app_D (cd.(code) (inr  c))
-               end;
+               match split_fin_sum l with
+               | inl iac => match split_fin_sum iac with
+                           | inl ia => _app_B (ab.(code) (L _ ia))
+                           | inr ic => _app_D (cd.(code) (L _ ic))
+                           end
+               | inr ac => match split_fin_sum ac with
+                          | inl a => _app_B (ab.(code) (R _ a))
+                          | inr c => _app_D (cd.(code) (R _ c))
+                          end
+               end
   |}.
 
-(** Rename visible program labels.
-    Having chosen to represent labels as binary trees encoded in [Type],
-    we, for instance, typically need to rename our visible labels through
-    associators.
-    The following generic combinator allow any relabelling. 
- *)
-Definition relabel_asm {A B C D} (f : A -> B) (g : C -> D)
+(** Rename visible program labels. *)
+Definition relabel_asm {A B C D} (f : FinC A B) (g : FinC C D)
            (bc : asm B C) : asm A D :=
-  {| code := relabel_bks (bimap id f) (bimap id g) bc.(code);
-  |}.
+  {| code := relabel_bks (bimap id f) (bimap id g)  bc.(code); |}.
 
-(** Labels that are exposed both as entry and exit points can be internalized.
-    This operation can be seen as linking two programs internal to [ab] together.
- *)
+(** Link labels from two programs together. *)
 Definition link_asm {I A B} (ab : asm (I + A) (I + B)) : asm A B :=
   {| internal := ab.(internal) + I;
      code := relabel_bks assoc_r assoc_l ab.(code);
   |}.
 
-(* ================================================================= *)
 (** ** Correctness *)
-(** We show the combinators correct by proving that their denotation
-    map to their [ktree] counterparts.
-    Since these combinators are the basic blocks we'll use in the
-    compiler to link compiled subterms, these correctness lemmas
-    will provide an equational theory sufficient to conduct
-    all needed reasoning.
-    Interestingly, [ktree] provides a sufficiently rich theory to
-    prove all these results involving [denote_asm], which is expressed
-    as a [loop], equationally.
- *)
+(** The combinators above map to their denotational counterparts. *)
 
-(* begin hide *)
+(* TODO: don't import stuff in the middle of modules *)
+From ExtLib Require Import
+     Structures.Monad.
 Import MonadNotation.
+From ITree Require Import
+     ITree KTree KTreeFacts.
 Import ITreeNotations.
 Import CatNotations.
 Local Open Scope cat.
-(* end hide *)
+
+Require Import Imp. (* TODO: remove this *)
 
 Section Correctness.
 
-  (** We reason about the denotation of [asm] programs, we therefore
-   need an appropriate domain of events [E]. *)
-  Context {E : Type -> Type}.
-  Context {HasLocals : Locals -< E}.
-  Context {HasMemory : Memory -< E}.
-  Context {HasExit : Exit -< E}.
+Context {E : Type -> Type}.
+Context {HasLocals : Locals -< E}.
+Context {HasMemory : Memory -< E}.
+Context {HasExit : Exit -< E}.
 
-  (** *** Internal structures *)
+(** *** Internal structures *)
 
-  (** Commutes denotation an [fmap] *)
-  Lemma fmap_block_map:
-    forall  {L L'} b (f: L -> L'),
-      denote_block (fmap_block f b) ≅ ITree.map f (denote_block b).
-  Proof.
-    (* Induction over the structure of the [block b] *)
-    induction b as [i b | br]; intros f.
-    - (* If it contains an instruction (inductive case). *)
-      simpl.
-      unfold ITree.map; rewrite bind_bind.
-      eapply eq_itree_bind; [| reflexivity].
-      intros []; apply IHb.
-    - (* If it's a jump, we consider the three cases. *)
-      simpl.
-      destruct br; simpl.
-      + unfold ITree.map; rewrite bind_ret; reflexivity.
-      + unfold ITree.map; rewrite bind_bind. 
-        eapply eq_itree_bind; [| reflexivity].
-        intros ?.
-        flatten_goal; rewrite bind_ret; reflexivity.
-      + rewrite (itree_eta (ITree.map _ _)).
-        cbn. apply eq_itree_Vis. intros [].
-  Qed.
+Lemma fmap_block_map:
+  forall  {L L'} b (f: FinC L L'),
+    denote_block (fmap_block f b) ≅ ITree.map f (denote_block b).
+Proof.
+  induction b as [i b | br]; intros f.
+  - simpl.
+    unfold ITree.map; rewrite bind_bind.
+    eapply eq_itree_eq_bind; try reflexivity.
+    intros []; apply IHb.
+  - simpl.
+    destruct br; simpl.
+    + unfold ITree.map; rewrite bind_ret; reflexivity.
+    + unfold ITree.map; rewrite bind_bind. 
+      eapply eq_itree_eq_bind; try reflexivity.
+      intros ?.
+      flatten_goal; rewrite bind_ret; reflexivity.
+    + rewrite (itree_eta (ITree.map _ _)).
+      cbn. apply eq_itree_Vis. intros [].
+Qed.
 
-  (** Denotes a list of instruction by binding the resulting trees. *)
-  Definition denote_list: list instr -> itree E unit :=
-    traverse_ denote_instr.
+Definition denote_list: list instr -> itree E unit :=
+  traverse_ denote_instr.
 
-  (** Correctness of the [after] operator.
-      Its denotation bind the denotation of the instructions
-      with the one of the branch.
-   *)
-  Lemma after_correct :
-    forall {label: Type} instrs (b: branch label),
-      denote_block (after instrs b) ≅ (denote_list instrs ;; denote_branch b).
-  Proof.
-    induction instrs as [| i instrs IH]; intros b.
-    - simpl; rewrite bind_ret; reflexivity.
-    - simpl; rewrite bind_bind.
-      eapply eq_itree_bind; try reflexivity.
-      intros []; apply IH.
-  Qed.
+Lemma after_correct :
+  forall {label: nat} instrs (b: branch (Fin.t label)),
+    denote_block (after instrs b) ≅ (denote_list instrs ;; denote_branch b).
+Proof.
+  induction instrs as [| i instrs IH]; intros b.
+  - simpl; rewrite bind_ret; reflexivity.
+  - simpl; rewrite bind_bind.
+    eapply eq_itree_eq_bind; try reflexivity.
+    intros []; apply IH.
+Qed.
 
-  (** Utility: denoting the [app] of two lists of instructions binds the denotations. *)
-  Lemma denote_list_app:
-    forall is1 is2,
-      @denote_list (is1 ++ is2) ≅ (@denote_list is1;; denote_list is2).
-  Proof.
-    intros is1 is2; induction is1 as [| i is1 IH]; simpl; intros; [rewrite bind_ret; reflexivity |].
-    rewrite bind_bind; setoid_rewrite IH; reflexivity.
-  Qed.
+Lemma denote_list_app:
+  forall is1 is2,
+    @denote_list (is1 ++ is2) ≅
+                 (@denote_list is1;; denote_list is2).
+Proof.
+  intros is1 is2; induction is1 as [| i is1 IH]; simpl; intros; [rewrite bind_ret; reflexivity |].
+  rewrite bind_bind; setoid_rewrite IH; reflexivity.
+Qed.
 
-  (** Correctness of the [raw_asm] operator.
-      Its denotation is the same as the denotation of the block.
-      Since it is hybrid between the level of [ktree]s (asm) and
-      [itree]s (block), the correctness is established at both
-      level for convenience.
-      Note that the ⩯ notation in the scope of [ktree] desugars to [eutt_ktree],
-      i.e. pointwise [eutt eq].
-   *)
-  Lemma raw_asm_block_correct_lifted {A} (b : block A) :
-    denote_asm (raw_asm_block b) ⩯
-               ((fun _ : unit => denote_block b) : ktree _ _ _).
-  Proof.
-    unfold denote_asm.
-    rewrite vanishing_ktree.
-    rewrite case_l_ktree', case_l_ktree.
-    unfold denote_b; simpl.
-    intros [].
-    rewrite fmap_block_map, map_map.
-    unfold ITree.map.
-    rewrite <- (bind_ret2 (denote_block b)) at 2.
-    reflexivity.
-  Qed.
 
-  Lemma raw_asm_block_correct {A} (b : block A) :
-    (denote_asm (raw_asm_block b) tt) ≈ (denote_block b).
-  Proof.
-    apply raw_asm_block_correct_lifted.
-  Qed.
+Lemma raw_asm_block_correct_lifted {A} (b : block (Fin.t A)) :
+   denote_asm (raw_asm_block b) ⩯
+          ((fun _ => denote_block b) : ktree _ _ _).
+Proof.
+  unfold denote_asm. simpl.
+  rewrite vanishing_Label.
+  rewrite case_l_Label'.
+  setoid_rewrite case_l_Label .
+  unfold denote_b; simpl.
+  reflexivity.
+Qed.
 
-  (** *** [asm] combinators *)
+Lemma raw_asm_block_correct {A} (b : block (t A)) :
+  eutt eq (denote_asm (raw_asm_block b) F1)
+          (denote_block b).
+Proof.
+  apply raw_asm_block_correct_lifted.
+Qed.
 
-  (** Correctness of the [pure_asm] combinator.
-      Its denotation is the lifting of a pure function
-      into a [ktree].
-   *)
-  Theorem pure_asm_correct {A B} (f : A -> B) :
-    denote_asm (pure_asm f) ⩯ @lift_ktree E _ _ f.
-  Proof.
-    unfold denote_asm .
-    rewrite vanishing_ktree. (* a pure_asm contains no internal label: we can remove them from the loop *)
-    rewrite case_l_ktree', case_l_ktree.
-    unfold denote_b; simpl.
-    intros ?.
-    rewrite map_ret.
-    reflexivity.
-  Qed.
+(** *** [asm] combinators *)
 
-  (** The identity gets denoted as the identity. *)
-  Theorem id_asm_correct {A} :
+Theorem pure_asm_correct {A B} (f : FinC A B) :
+    denote_asm (pure_asm f)
+  ⩯ @lift_ktree E _ _ f.
+Proof.
+  unfold denote_asm .
+  rewrite vanishing_Label.
+  rewrite case_l_Label'.
+  setoid_rewrite case_l_Label.
+  unfold denote_b; simpl.
+  intros ?.
+  reflexivity.
+Qed.
+
+Definition id_asm_correct {A} :
     denote_asm (pure_asm id)
-               ⩯ id_ A.
-  Proof.
-    rewrite pure_asm_correct; reflexivity.
-  Defined.
+  ⩯ id_ A.
+Proof.
+  rewrite pure_asm_correct; reflexivity.
+Defined.
 
-  (** Correctness of the [app_asm] combinator.
-      The resulting [asm] gets denoted to the bimap of its subcomponent.
-      The proof is a bit more complicated. It makes a lot more sense if drawn.
-   *)
-  Theorem app_asm_correct {A B C D} (ab : asm A B) (cd : asm C D) :
-    denote_asm (app_asm ab cd)
-               ⩯ bimap (denote_asm ab) (denote_asm cd).
-  Proof.
-    unfold denote_asm.
-    (*
-      On the left-hand-side, we have a [loop] of two [asm] mashed together.
-      On the right-hand-side however we have two [loop]s combined together.
-      The game is to massage them through successive rewriting until they
-      line up.
-     *)
+Lemma fwd_eqn {a b : Type} (f g : ktree E a b) :
+  (forall h, h ⩯ f -> h ⩯ g) -> f ⩯ g.
+Proof.
+  intro H; apply H; reflexivity.
+Qed.
 
-    (* We first work on the rhs to reduce it to a single loop.
-       The textual explanations are fairly cryptic. The key intuition comes
-       by drawing the state of the circuit and using the rewiring laws
-       the categorical structure provides, as represented for instance here:
-       https://en.wikipedia.org/wiki/Traced_monoidal_category
-       [bimap_ktree_loop] and [loop_bimap_ktree] are the _superposing_ laws.
-       [compose_loop] and [loop_compose] are the _naturality_ in _X_ and _Y_.
-       [loop_loop] is the second _vanishing_ law.
-     *)
-    match goal with | |- ?x ⩯ _ => set (lhs := x) end.
-    rewrite bimap_ktree_loop. (* a loop superposed atop another diagram can englob the latter *)
-    rewrite loop_bimap_ktree. (* as well as if the loop is under... But it takes a bit more rewiring! *)
-    rewrite <- compose_loop.   (* a loop append to diagrams can swallow them... *)
-    rewrite <- loop_compose.   (* ... from either side. *)
-    rewrite loop_loop.        (* Finally, two nested loop can be combined. *)
+Lemma cat_eq2_l {a b c : Type} (h : ktree E a b) (f g : ktree E b c) :
+  f ⩯ g -> h >>> f ⩯ h >>> g.
+Proof.
+  intros H; rewrite H; reflexivity.
+Qed.
 
-    subst lhs.
-    (* Remain now to relate the bodies of the loops on each side. *)
-    (* First by some more equational reasoning. *)
-    rewrite <- (loop_rename_internal' swap swap).
-    2: apply swap_involutive; typeclasses eauto.
-    apply eq_ktree_loop.
-    rewrite !cat_assoc; try typeclasses eauto.
-    rewrite <- !sym_ktree_unfold, !assoc_l_ktree, !assoc_r_ktree, !bimap_lift_id, !bimap_id_lift, !compose_lift_ktree_l, compose_lift_ktree.
+Lemma cat_eq2_r {a b c : Type} (h : ktree E b c) (f g : ktree E a b) :
+  f ⩯ g -> f >>> h ⩯ g >>> h.
+Proof.
+  intros H; rewrite H; reflexivity.
+Qed.
 
-    (* And finally a case analysis on the label provided. *)
-    unfold cat, Cat_ktree, ITree.cat, lift_ktree.
-    intro x. rewrite bind_ret; simpl.
-    destruct x as [[|]|[|]]; cbn.
-    (* ... *)
-    all: unfold cat, Cat_ktree, ITree.cat.
-    all: try rewrite bind_bind.
-    all: unfold _app_B, _app_D.
-    all: rewrite fmap_block_map.
-    all: unfold ITree.map.
-    all: apply eutt_bind; try reflexivity.
-    all: intros []; rewrite (itree_eta (ITree.bind _ _)); cbn; reflexivity.
-  Qed.
+Lemma local_rewrite1 {a b c : Type}:
+    bimap (id_ a) (@swap _ (ktree E) _ _ b c) >>> assoc_l >>> swap
+  ⩯ assoc_l >>> bimap swap (id_ c) >>> assoc_r.
+Proof.
+  symmetry.
+  apply fwd_eqn; intros h Eq.
+  do 2 apply (cat_eq2_l (bimap (id_ _) swap)) in Eq.
+  rewrite <- cat_assoc, bimap_cat, swap_involutive, cat_id_l,
+    bimap_id, cat_id_l in Eq.
+  rewrite <- (cat_assoc _ _ _ assoc_r), <- (cat_assoc _ _ assoc_l _)
+    in Eq.
+  rewrite <- swap_assoc_l in Eq.
+  rewrite (cat_assoc _ _ _ assoc_r) in Eq.
+  rewrite assoc_l_mono in Eq.
+  rewrite cat_id_r in Eq.
+  rewrite cat_assoc.
+  assumption.
+  all: typeclasses eauto.
+Qed.
 
-  (** Correctness of the [relabel_asm] combinator.
-      Its denotation is the same as denoting the original [asm],
-      and composing it on both sides with the renaming functions
-      lifted as [ktree]s.
-   *)
-  Lemma relabel_bks_correct {A B C D} (f : A -> B) (g : C -> D)
-             (bc : bks B C) :
+Lemma local_rewrite2 {a b c : Type}:
+    swap >>> assoc_r >>> bimap (id_ _) swap
+  ⩯ @assoc_l _ (ktree E) _ _ a b c >>> bimap swap (id_ _) >>> assoc_r.
+Proof.
+  symmetry.
+  apply fwd_eqn; intros h Eq.
+  do 2 apply (cat_eq2_r (bimap (id_ _) swap)) in Eq.
+  rewrite cat_assoc, bimap_cat, swap_involutive, cat_id_l,
+    bimap_id, cat_id_r in Eq.
+  rewrite 2 (cat_assoc _ assoc_l) in Eq.
+  rewrite <- swap_assoc_r in Eq.
+  rewrite <- 2 (cat_assoc _ assoc_l) in Eq.
+  rewrite assoc_l_mono, cat_id_l in Eq.
+  assumption.
+  all: try typeclasses eauto.
+Qed.
+
+Lemma loop_bimap_ktree {I A B C D}
+      (ab : ktree E A B) (cd : ktree E (I + C) (I + D)) :
+    bimap ab (loop cd)
+  ⩯ loop (assoc_l >>> bimap swap (id_ _)
+                  >>> assoc_r
+                  >>> bimap ab cd
+                  >>> assoc_l >>> bimap swap (id_ _) >>> assoc_r).
+Proof.
+  rewrite swap_bimap, bimap_ktree_loop.
+  rewrite <- compose_loop, <- loop_compose.
+  rewrite (swap_bimap _ _ cd ab).
+  rewrite <- !cat_assoc.
+  rewrite local_rewrite1.
+  rewrite 2 cat_assoc.
+  rewrite <- (cat_assoc _ swap assoc_r).
+  rewrite local_rewrite2.
+  rewrite <- !cat_assoc.
+  reflexivity.
+  all: typeclasses eauto.
+Qed.
+
+Definition app_asm_correct {A B C D} (ab : asm A B) (cd : asm C D) :
+     denote_asm (app_asm ab cd)
+  ⩯ bimap (denote_asm ab) (denote_asm cd).
+Proof.
+  unfold denote_asm.
+
+  match goal with | |- ?x ⩯ _ => set (lhs := x) end.
+  rewrite bimap_Label_loop.
+  (*
+  rewrite loop_bimap_ktree.
+  rewrite <- compose_loop.
+  rewrite <- loop_compose.
+  rewrite loop_loop.
+  subst lhs.
+  rewrite <- (loop_rename_internal' swap swap).
+  2: apply swap_involutive; typeclasses eauto.
+  apply eq_ktree_loop.
+  rewrite !cat_assoc.
+  rewrite <- !sym_ktree_unfold, !assoc_l_ktree, !assoc_r_ktree, !bimap_lift_id, !bimap_id_lift, !compose_lift_ktree_l, compose_lift_ktree.
+  unfold cat, Cat_ktree, ITree.cat, lift_ktree.
+  intro x. rewrite bind_ret; simpl.
+  destruct x as [[|]|[|]]; cbn.
+  (* ... *)
+  all: unfold cat, Cat_ktree, ITree.cat.
+  all: try typeclasses eauto.
+  all: try rewrite bind_bind.
+  all: unfold _app_B, _app_D.
+  all: rewrite fmap_block_map.
+  all: unfold ITree.map.
+  all: apply eutt_bind; try reflexivity.
+  all: intros []; rewrite (itree_eta (ITree.bind _ _)); cbn; reflexivity.
+Qed.
+*)
+Admitted.
+
+Definition relabel_bks_correct {A B C D} (f : FinC A B) (g : FinC C D)
+           (bc : bks B C) :
     denote_b (relabel_bks f g bc)
-             ⩯ lift_ktree f >>> denote_b bc >>> lift_ktree g.
-  Proof.
-    rewrite lift_compose_ktree.
-    rewrite compose_ktree_lift.
-    intro a.
-    unfold denote_b, relabel_bks.
-    rewrite fmap_block_map.
-    reflexivity.
-  Qed.
-
-  Theorem relabel_asm_correct {A B C D} (f : A -> B) (g : C -> D)
-             (bc : asm B C) :
-    denote_asm (relabel_asm f g bc)
-               ⩯ lift_ktree f >>> denote_asm bc >>> lift_ktree g.
-  Proof.
-    unfold denote_asm.
-    simpl.
-    rewrite relabel_bks_correct.
-    rewrite <- compose_loop.
-    rewrite <- loop_compose.
-    apply eq_ktree_loop.
-    rewrite !bimap_id_lift.
-    reflexivity.
-  Qed.
-
-  (** Correctness of the [link_asm] combinator.
-      Linking is exactly looping, it hides internal labels/wires.
+  ⩯ lift_ktree f >>> denote_b bc >>> lift_ktree g.
+Proof.
+  (*
+  rewrite lift_compose_ktree.
+  rewrite compose_ktree_lift.
+  intro a.
+  unfold denote_b, relabel_bks.
+  rewrite fmap_block_map.
+  reflexivity.
+Qed.
    *)
-  Theorem link_asm_correct {I A B} (ab : asm (I + A) (I + B)) :
-    denote_asm (link_asm ab) ⩯ loop (denote_asm ab).
-  Proof.
-    unfold denote_asm.
-    rewrite loop_loop.
-    apply eq_ktree_loop.
-    simpl.
-    rewrite relabel_bks_correct.
-    rewrite <- assoc_l_ktree, <- assoc_r_ktree.
-    reflexivity.
-  Qed.
+Admitted.
+
+Definition relabel_asm_correct {A B C D} (f : FinC A B) (g : FinC C D)
+           (bc : asm B C) :
+    denote_asm (relabel_asm f g bc)
+  ⩯ lift_ktree f >>> denote_asm bc >>> lift_ktree g.
+Proof.
+  (*
+  unfold denote_asm.
+  simpl.
+  rewrite relabel_bks_correct.
+  rewrite <- compose_loop.
+  rewrite <- loop_compose.
+  apply eq_ktree_loop.
+  rewrite !bimap_id_lift.
+  reflexivity.
+Qed.
+   *)
+Admitted.
+
+Definition link_asm_correct {I A B} (ab : asm (I + A) (I + B)) :
+    denote_asm (link_asm ab) ⩯ loop_Label (denote_asm ab).
+Proof.
+  unfold denote_asm.
+  (*
+  rewrite loop_loop.
+  apply eq_ktree_loop.
+  simpl.
+  rewrite relabel_bks_correct.
+  rewrite <- assoc_l_ktree, <- assoc_r_ktree.
+  reflexivity.
+Qed.
+*)
+Admitted.
 
 End Correctness.
-
-(** We have defined four low-level combinators allowing us to combine [asm]
-    programs together. These combinators are correct in the sense that
-    their denotation is bisimilar to their denotational counterparts at the
-    [ktree] level.
-    This theory of linking is only tied to _Asm_, and can therefore be reused
-    either for other compilers targetting Asm, or for optimizations over Asm. 
-    We now turn to its specific use to finally define our compiler, defined
-    in [Imp2Asm.v].
- *)
