tutorial/Imp2Asm.v
@@ -1,55 +1,40 @@
-(** * Compilation of Imp to Asm *)
-
-(** We are now ready to define our compiler.
-    The compilation of [expr]essions is of no interest.
-    The interesting part is in the structure of the
-    compilation of instructions: we build higher level
-    [asm] combinators from the primitive ones defined
-    in [AsmCombinators.v]. Each of these combinator
-    transcribes a control flow construct of the _Imp_
-    language as a linking operation over _Asm_.
-    Their correctness will be shown in the same style as
-    the elementary combinators, isolating the control
-    flow reasoning.
-    Additionnaly, although naturally their choice here
-    is tied to _Imp_, they are fairly generic constructs
-    and could therefore be reused.
-*)
-
-(* begin hide *)
 Require Import Imp Asm Utils_tutorial AsmCombinators.
 
 Require Import Psatz.
 
 From Coq Require Import
-     Strings.String.
+     Strings.String
+     Morphisms
+     Setoid
+     Decimal
+     Numbers.DecimalString
+     Vectors.Fin
+     ZArith
+     RelationClasses.
 
 From ITree Require Import
+     Basics.Category
+     Basics.Function
+     Effects.Env
      ITree.
+
+From ExtLib Require Import
+     Core.RelDec
+     Structures.Monad
+     Structures.Maps
+     Programming.Show
+     Data.Map.FMapAList.
 
 Import ListNotations.
 Open Scope string_scope.
-(* end hide *)
-
-(* ================================================================= *)
-(** ** Compilation of expressions *)
 
 Section compile_assign.
-
-  (** We use a simple scheme to ensure disjointness of user variables from local
-  ones introduced by the compiler: the former ones get prefix by "temp_", the latter
-  ones by "local_". *)
 
   Definition gen_tmp (n: nat): string :=
     "temp_" ++ string_of_nat n.
 
   Definition varOf (s : var) : var := "local_" ++ s.
 
-  (** Expressions are compiled straightforwardly.
-      The argument [l] is the number of local variables already introduced to compile
-      the expression, and is used for the name of the next one.
-      The result of the computation [compile_expr l e] always ends up stored in [gen_tmp l]. 
-   *)
   Fixpoint compile_expr (l: nat) (e: expr): list instr :=
     match e with
     | Var x => [Imov (gen_tmp l) (Ovar (varOf x))]
@@ -68,36 +53,22 @@ Section compile_assign.
       instrs1 ++ instrs2 ++ [Imul (gen_tmp l) (gen_tmp l) (Ovar (gen_tmp (1 + l)))]
       end.
 
-  (** Compiles the expression and then move the result (in [gen_tmp 0]) to the mangled variable. *)
   Definition compile_assign (x: Imp.var) (e: expr): list instr :=
     let instrs := compile_expr 0 e in
     instrs ++ [Imov (varOf x) (Ovar (gen_tmp 0))].
 
 End compile_assign.
 
-(* ================================================================= *)
-(** ** Control flow combinators *)
-
-
 (** Sequencing of blocks: the program [seq_asm ab bc] links the
     exit points of [ab] with the entry points of [bc].
-    
+
 [[
            B
    A---ab-----bc---C
 ]]
 
-   ... can be implemented using just [app_asm], [relabel_asm] and [link_asm].
+   ... can be implemented using just [app_asm] and [link_asm].
 
-  Indeed, [app_asm ab bc] can be visualized as:
-[[
-  A---ab---B
-  B---bc---C
-]]
- i.e. a [asm (A + B) (B + C)]. To link them, we need first to swap the entry points.
-
-We obtain the following diagram:
-[seq_asm ab bc]
 [[
        +------+
        |      |
@@ -105,55 +76,33 @@ We obtain the following diagram:
        |
       B+--bc------C
 ]]
-
-Which translates to:
- *)
+*)
 Definition seq_asm {A B C} (ab : asm A B) (bc : asm B C): asm A C :=
   link_asm (relabel_asm swap (id_ _) (app_asm ab bc)).
 
-
-(** Location of temporary for [if]. *)
+(* Location of temporary for [if]. *)
 Definition tmp_if := gen_tmp 0.
 
-(** Turns the list of instructions resulting from the conditional
-    expression of a _if_ to a block with two exit points.
- *)
-Definition cond_asm (e : list instr) : asm unit (unit + unit) :=
-  raw_asm_block (after e (Bbrz tmp_if (inr tt) (inl tt))).
+(* Conditional *)
+Definition cond_asm (e : list instr) : asm 1 2 :=
+  raw_asm_block (after e (Bbrz tmp_if F1 (FS F1))).
 
-(** Conditional branch of blocks.
-    The program [if_asm e tp fp] creates a block out of [e] jumping
-    either left or right.
-    Using [seq_asm], this block is sequenced with the vertical
-    composition [app_asm] of [tp] and [fp].
-    Remains one mismatch: [app_asm] duplicates the domain of outputs,
-    although they share the same. We hence use [relabel_asm] to collapse
-    them together.
-
- [if_asm e tp fp]
+(** [if_asm e tp fp]
 [[
            true
-       /ee-------tp---A\
-    1--                 --A
-       \ee-------fp---A/
+        ee-------tp---C
+    1---ee-------fp---C
            false
 ]]
  *)
 Definition if_asm {A}
-           (e : list instr) (tp : asm unit A) (fp : asm unit A) :
-  asm unit A :=
+           (e : list instr) (tp : asm 1 A) (fp : asm 1 A) :
+  asm 1 A :=
   seq_asm (cond_asm e)
           (relabel_asm (id_ _) merge (app_asm tp fp)).
 
-(* Conditional looping of blocks.
-   The program [while_asm e p] composes vertically two programs:
-   an [if_asm] construct with [p] followed by a jump on the true branch,
-   and a unique jump on the false branch. 
-   The loop is then closed with [link_asm] by matching the jump from the
-   true branch to the entry point.
-
-[while_asm e p]
-[[
+(* [while_asm e p]
+/[[
       +-------------+
       |             |
       |    true     |
@@ -162,28 +111,19 @@ Definition if_asm {A}
            false
 ]]
 *)
-Definition while_asm (e : list instr) (p : asm unit unit) :
-  asm unit unit :=
+Definition while_asm (e : list instr) (p : asm 1 1) :
+  asm 1 1 :=
   link_asm (relabel_asm (id_ _) merge
     (app_asm (if_asm e
-                (relabel_asm id inl p)
-                (pure_asm inr))
-            (pure_asm inl))).
+                (relabel_asm id inl_ p)
+                (pure_asm inr_))
+            (pure_asm inl_))).
 
-(** Equipped with our combinators, the compiler writes itself
-    by induction on the structure of the statement.
-*)
-Fixpoint compile (s : stmt) {struct s} : asm unit unit :=
+Fixpoint compile (s : stmt) {struct s} : asm 1 1 :=
   match s with
   | Skip => id_asm
-  | Assign x e => raw_asm_block (after (compile_assign x e) (Bjmp tt))
+  | Assign x e => raw_asm_block (after (compile_assign x e) (Bjmp F1))
   | Seq l r => seq_asm (compile l) (compile r)
   | If e l r => if_asm (compile_expr 0 e) (compile l) (compile r)
   | While e b => while_asm (compile_expr 0 e) (compile b)
   end.
-
-(** We now consider its proof of correctness in [Imp2AsmCorrectness.v]. *)
-
-
-
-
